@prefix rdf:    	<http://www.w3.org/1999/02/22-rdf-syntax-ns#> .
@prefix owl:    	<http://www.w3.org/2002/07/owl#> .
@prefix rdfs:   	<http://www.w3.org/2000/01/rdf-schema#> .
@prefix xsd:    	<http://www.w3.org/2001/XMLSchema#> .
@prefix dcterms:	<http://purl.org/dc/terms/> .
@prefix voaf:   	<http://purl.org/vocommons/voaf#> .
@prefix foaf:   	<http://xmlns.com/foaf/0.1/> .
@prefix dce:    	<http://purl.org/dc/elements/1.1/> .
@prefix bot:		<https://w3id.org/bot#>
@prefix geo:		<http://www.opengis.net/ont/geosparql#>

@prefix stg: <https://github.com/JWerbrouck/Thesis/stg.ttl> .

voaf:Vocabulary a owl:Class .
dcterms:title a owl:AnnotationProperty .
dcterms:description a owl:AnnotationProperty .
dcterms:issued a owl:AnnotationProperty .
dcterms:modified a owl:AnnotationProperty .
dcterms:creator a owl:AnnotationProperty .
dcterms:contributor a owl:AnnotationProperty .
dcterms:license a owl:AnnotationProperty .
foaf:Person a owl:Class .
foaf:name a owl:DatatypeProperty .

#################################
# METADATA
#################################
<https://github.com/JWerbrouck/Thesis/stg#> rdf:type voaf:Vocabulary , 
                                 owl:Ontology ;
    dce:modified "Mai 3rd 2018"^^xsd:string ;
    owl:versionInfo "Mai 3rd 2018"^^xsd:string ;
    dcterms:issued "June 1st 2018"^^xsd:date ;
	dcterms:creator [a foaf:Person ; foaf:name "Jeroen Werbrouck" ] ;
    dcterms:title "STG: Scan-to-Graph"@en ;
    dcterms:description """Scan-to-Graph (STG) is a simple vocabulary defining some concepts for linking instances with their geometry serialized in a certain format.
It is meant as an aid for point-cloud based reconstruction of heritage or renovation projects, within a Linked Data context.
    
#################################
# CLASSES
#################################
stg:RepresentingDocument a owl:Class ;
		rdfs:label		"File with geometrical representation"@en ,
			"Bestand met geometrie"@nl ;
		
		rdfs:comment	"A file that contains a geometrical representation of the whole or a part of the whole."@en ,
						"Een bestand dat een geometrische representatie van het geheel of van een deel ervan bevat."@nl .

stg:SourceFile a owl:Class ;
		rdfs:label		"Source"@en ,
			"Bron"@nl ;
		rdfs:comment	"File that contains information about the real-world object and can serve as a modelling source."@en ,
						"Bestand met informatie over het reÃ«le object, dat kan dienen als bronmateriaal bij het modelleren."@nl ;
		
		rdfs:subClassOf 	stg:RepresentingDocument.
		
stg:PointCloudFile a owl:Class ;
		rdfs:subClassOf stg:SourceFile ;
        
		rdfs:label      "Pointcloudfile"@en ,
			"Puntwolkdocument"@nl ;
        
        rdfs:comment    "Refers to an external point cloud file that represents the instance geometrically."@en ,
                        "Verwijst naar een extern puntwolkbestand dat het voorwerp geometrisch representeert."@nl .
						
stg:RhinoFile a owl:Class ;.
		rdfs:subClassOf stg:RepresentingDocument ;
        
		rdfs:label      ".3dm file"@en ,
			".3dm bestand"@nl ;
        
        rdfs:comment    "Refers to an external Rhinoceros (McNeel) document (.3dm) that contains a geometrical representation of the whole model or parts of it."@en ,
                        "Verwijst naar een extern Rhinoceros (McNeel) document (.3dm) dat een geometrische representatie van het gehele model of delen ervan bevat."@nl .						
			
stg:STEPRepresentation a rdfs:Literal ;
        rdfs:label      "STEP Literal"@en ,
			"STEPLiteral"@nl ;
        
        rdfs:comment    "A Literal that contains the raw STEP ("Standard for the Exchange of Product model data") representation of the instance."@en ,
                        "Een 'Literal' die de ruwe data van de STEP ("Standard for the Exchange of Product model data") representatie van het voorwerp."@nl .

stg:OBJRepresentation a rdfs:Literal ;
        rdfs:label      "OBJ Literal"@en ,
			"OBJ Literal"@nl ;
        
        rdfs:comment    "A Literal that contains the raw OBJ (mesh) representation of the instance."@en ,
                        "Een 'Literal' die de ruwe data van de OBJ (mesh) representatie van het voorwerp bevat."@nl .
						
stg:RhinoID a rdfs:Datatype ;
        rdfs:label      "Literal containing Rhino-ID"@en ,
			"Literal met Rhino-ID"@nl ;
        
        rdfs:comment    "A Literal (as datatype) that encapsulates a Rhino-ID that identifies an object representation in an stg:RhinoDocument."@en ,
                        "Een Literal (as datatype) die een Rhino-ID bevat dat een objectrepresentatie in een stg:RhinoDocument identificeert."@nl.
						
#################################
# OBJECT PROPERTIES
#################################

stg:hasRepresentingFile a owl:ObjectProperty ;
        rdfs:label      "Document with geometry"@en ,
			"Document met geometrie"@nl ;
        
	rdfs:comment    "Relates an instance to a document that is its geometrical representation"@en ,
        		"Relateert een objectinstantie aan een document dat dit geometrisch representeert"@nl ;
        
        rdfs:range  	stg:RepresentingDocument.

stg:hasRhinoFile a owl:ObjectProperty ;
        rdfs:label      "has Rhino File"@en ,
			"heeft Rhino bestand"@nl ;

	rdfs:comment    "Connects an instance with an external Rhino (.3dm) file that contains its geometry."@en ,
                    "Verbindt een instantie met een extern Rhino (.3dm) document dat de geometrie van dit element bevat"@nl ;
        
		rdfs:subPropertyOf	stg:hasRepresentingFile ;
		
        rdfs:range      stg:RhinoFile .

stg:hasPointCloudFile a owl:ObjectProperty ;
        rdfs:label      "has Point Cloud File"@en ,
			"heeft Puntwolkbestand"@nl ;

	rdfs:comment    "Connects an instance with an external Point Cloud file that contains its geometry."@en ,
                    "Verbindt een instantie met een externe puntwolk die de geometrie van dit element bevat"@nl ;
        
		rdfs:subPropertyOf	stg:hasRepresentingFile ;
		
        rdfs:range      stg:PointCloudFile.		
		
stg:asSTEP	a	owl:DatatypeProperty;
		rdfs:label		"as STEP"@en ,
			"als STEP"@nl ;
		
	rdfs:comment	"connects an instance with a Literal containing its raw STEP serialization"@en ,
					"Verbindt een instantie met een Literal die de ruwe STEP-serializatie ervan behelst"@nl ;
					
	rdfs:subPropertyOf	geo:hasSerialization ;
	
	rdfs:domain		geo:Geometry ;
	rdfs:range		stg:STEPRepresentation .
	
stg:asOBJ	a	owl:DatatypeProperty ;
		rdfs:label		"as OBJ"@en ,
			"als OBJ"@nl ;
		
	rdfs:comment	"connects an instance with a Literal containing its raw OBJ serialization"@en ,
					"Verbindt een instantie met een Literal die de ruwe OBJ-serializatie ervan behelst"@nl ;
					
	rdfs:subPropertyOf	geo:hasSerialization ;
	
	rdfs:domain		geo:Geometry ;
	rdfs:range		stg:OBJRepresentation .

stg:hasRhinoID	a	owl:DatatypeProperty ;
		rdfs:label		"reference to RhinoID"@en ,
			"refereert naar RhinoID"@nl ;
		
	rdfs:comment	"connects an instance with a Literal containing a RhinoID as a reference to the object representation in the stg:RhinoFile"@en ,
					"Verbindt een instantie met een Literal die de ruwe OBJ-serializatie ervan behelst"@nl ;
	
	rdfs:domain		geo:Geometry ;
	rdfs:range		stg:RhinoID .

stg:hasModellingRemark a owl:DatatypeProperty ;
	rdfs:label		"Modelling remark"@en ,
					"Modelleer opmerking"@nl ;
					
	rdfs:comment	"Statement about the geometry, such as metadata or an assumption that was made while modelling as-built geometry, based on ambiguous information provided by the sources, e.g. occlusions in a point cloud"@en ,
					"Opmerking over de geometrie, zoals metadata of een modelleerveronderstelling gebaseerd op onduidelijkheden in het bronmateriaal, bv. occlusies in een puntwolk."@nl ;
	
	rdfs:domain		geo:Geometry ;
	rdfs:range		rdfs:Literal .
