@prefix : 		<https://raw.githubusercontent.com/JWerbrouck/Thesis/master/stg.ttl#> .
@prefix rdf:    	<http://www.w3.org/1999/02/22-rdf-syntax-ns#> .
@prefix owl:    	<http://www.w3.org/2002/07/owl#> .
@prefix rdfs:   	<http://www.w3.org/2000/01/rdf-schema#> .
@prefix bot:		<https://w3id.org/bot#> .
@prefix xsd:    	<http://www.w3.org/2001/XMLSchema#> .
@prefix dcterms:	<http://purl.org/dc/terms/> .
@prefix voaf:   	<http://purl.org/vocommons/voaf#> .
@prefix foaf:   	<http://xmlns.com/foaf/0.1/> .
@prefix dce: 		<http://purl.org/dc/elements/1.1/> .
@prefix geo:		<http://www.opengis.net/ont/geosparql#> .
@prefix stg: 		<https://raw.githubusercontent.com/JWerbrouck/Thesis/master/stg.ttl#> .

#################################
# METADATA
#################################

<https://github.com/JWerbrouck/Thesis/blob/master/stg.ttl> rdf:type owl:Ontology ;
    dce:modified "May 3rd 2018"^^xsd:string ;
    owl:versionInfo "May 3rd 2018"^^xsd:string ;
    dcterms:issued "June 1st 2018"^^xsd:date ;
    dcterms:title "STG: Scan-to-Graph"@en ;
    dcterms:description """Scan-to-Graph (STG) is a simple vocabulary defining some concepts for linking instances with their geometry serialized in a certain format.
It is meant as an aid for point-cloud based reconstruction of heritage or renovation projects, within a Linked Data context."""@en .


#################################################################
#    Classes
#################################################################

stg:RepresentingFile a owl:Class ;
		rdfs:label	"File with geometrical representation"@en ,
				"Bestand met geometrie"@nl ;
		
		rdfs:comment	"A file that contains a geometrical representation of the whole or a part of the whole."@en ,
				"Een bestand dat een geometrische representatie van het geheel of van een deel ervan bevat."@nl .
stg:SourceFile 	a owl:Class ;
		rdfs:label	"Source"@en ,
				"Bron"@nl ;
		rdfs:comment	"File that contains information about the real-world object and can serve as a modelling source."@en ,
				"Bestand met informatie over het reÃ«le object, dat kan dienen als bronmateriaal bij het modelleren."@nl ;
		
		rdfs:subClassOf 	stg:RepresentingFile.						

stg:ReconstructedFile 	a owl:Class ;
		rdfs:label	"Reconstruction"@en ,
				"Reconstructie"@nl ;
		rdfs:comment	"File that was modelled based on real world sources."@en ,
				"Bestand gemodelleerd op basis van bronnen."@nl ;
		
		rdfs:subClassOf 	stg:RepresentingFile.	

stg:PointCloudFile 	a owl:Class ;
		rdfs:subClassOf 	stg:SourceFile ;
        
		rdfs:label      "Pointcloudfile"@en ,
				"Puntwolkdocument"@nl ;
        
        	rdfs:comment    "Refers to an external point cloud file that represents the instance geometrically (URI)."@en ,
                        	"Verwijst naar een extern puntwolkbestand dat het voorwerp geometrisch representeert (URI)."@nl .

stg:STEPFile 	rdf:type owl:Class ;
           	rdfs:subClassOf stg:ReconstructedFile ;

		rdfs:label 	"STEP file"@en ,
				"STEP bestand"@nl ;

           	rdfs:comment 	"Refers to a URI that gives acces to a STEP file."@en ,
				"Verwijst naar een URI die toegang tot een STEP bestand verschaft."@nl .

stg:RhinoFile 	rdf:type owl:Class ;
           	rdfs:subClassOf stg:ReconstructedFile ;

		rdfs:label 	".3dm file"@en ,
				".3dm bestand"@nl ;

           	rdfs:comment 	"Refers to an external Rhinoceros (McNeel) document (.3dm) that contains a geometrical representation of the whole model or parts of it."@en ,
				"Verwijst naar een extern Rhinoceros (McNeel) document (.3dm) dat een geometrische representatie van het gehele model of delen ervan bevat."@nl .

stg:RhinoID 	rdf:type rdfs:Datatype ;
        	rdfs:label      "Literal containing Rhino-ID"@en ,
				"Literal met Rhino-ID"@nl ;
        
        	rdfs:comment    "A Literal (as datatype) that encapsulates a Rhino-ID that identifies an object representation in an stg:RhinoDocument."@en ,
                        	"Een Literal (as datatype) die een Rhino-ID bevat dat een objectrepresentatie in een stg:RhinoDocument identificeert."@nl.		   
			
stg:STEPRepresentation 	rdf:type rdfs:DataType ;
        	rdfs:label      "STEP Literal"@en ,
				"STEP Literal"@nl ;

        	rdfs:comment    "A Literal that contains the raw STEP representation of the instance"@en ,
				"Een Literal die de STEP representatie van het object als ruwe data beschrijft"@nl .

stg:InternalGeometry	rdf:type owl:Class ;
		rdfs:label	"Internal Geometry"@en ;
		rdfs:comment	"Indicates whether a geometry is the part of an object contained in another object (e.g. part of a console is 'internal' in a wall)"@en .

stg:ProjectOrigin	rdf:type owl:Class ;
		rdfs:label	"Project Origin"@en ;
		rdfs:comment	"A geometry referring to the Project's Origin"@en ;
		rdfs:subClassOf	geo:Geometry .
		
stg:ModellingRemark	rdf:type owl:Class ;
		rdfs:label	"Modellingremark"@en ;
		rdfs:comment	"Something that contains information about a geometry"@en .

stg:Assumption	rdf:type owl:Class ;
		rdfs:label	"Assumption"@en ;
		rdfs:comment	"An assumption that contains information about a geometry"@en ;
		rdfs:subClassOf	stg:ModellingRemark .

stg:LevelOfAccuracy rdf:type owl:Class ;
		rdfs:label	"USIBD LOA"@en ;
		rdfs:comment	"States the (represented) LOA of a geometry after deviation analysis (definition according to USIBD LOA specification)"@en ;
		rdfs:subClassOf	stg:ModellingRemark .

stg:OccludedGeometry	rdf:type owl:Class ;
		rdfs:label		"Assumption"@en ;
		rdfs:comment	"Indicates whether a geometry contains an occluded area"@en ;
		rdfs:subClassOf	stg:ModellingRemark .

#################################
# OBJECT PROPERTIES
#################################

stg:hasRepresentingFile a owl:ObjectProperty ;
		rdfs:label      "Document with geometry"@en ,
				"Document met geometrie"@nl ;

		rdfs:comment    "Relates an instance to a document that is its geometrical representation"@en ,
				"Relateert een objectinstantie aan een document dat dit geometrisch representeert"@nl ;

		rdfs:range  	stg:RepresentingDocument.

stg:hasRhinoFile a owl:ObjectProperty ;
		rdfs:label      "has Rhino File"@en ,
				"heeft Rhino bestand"@nl ;

		rdfs:comment    "Connects an instance with an external Rhino (.3dm) file that contains its geometry."@en ,
			    	"Verbindt een instantie met een extern Rhino (.3dm) document dat de geometrie van dit element bevat"@nl ;
        
		rdfs:subPropertyOf	stg:hasRepresentingFile ;
		
        	rdfs:range      stg:RhinoFile .

stg:hasPointCloudFile a owl:ObjectProperty ;
		rdfs:label      "has Point Cloud File"@en ,
				"heeft Puntwolkbestand"@nl ;

		rdfs:comment    "Connects an instance with an external Point Cloud file that contains its geometry."@en ,
				"Verbindt een instantie met een externe puntwolk die de geometrie van dit element bevat"@nl ;

		rdfs:subPropertyOf	stg:hasRepresentingFile ;

		rdfs:range      stg:PointCloudFile .

stg:hasLocalVersion a owl:DataTypeProperty ;
		rdfs:label      "has Point Cloud File"@en ,
				"heeft Puntwolkbestand"@nl ;

		rdfs:comment    "Connects an instance with an external (local) file that contains its geometry."@en ,
				"Verbindt een instantie met een extern (lokaal) bestand dat de geometrie van dit element bevat"@nl ;

		rdfs:subPropertyOf	stg:hasRepresentingFile ;
		rdfs:domain	stg:PointCloudFile ;
		rdfs:range      rdfs:Literal .
		
stg:asSTEP	a	owl:DatatypeProperty;
		rdfs:label	"as STEP"@en ,
				"als STEP"@nl ;
		
		rdfs:comment	"connects an instance with a Literal containing its raw STEP serialization"@en ,
				"Verbindt een instantie met een Literal die de ruwe STEP-serializatie ervan behelst"@nl ;

		rdfs:subPropertyOf	geo:hasSerialization ;

		rdfs:domain		geo:Geometry ;
		rdfs:range		stg:STEPRepresentation .
	

stg:hasRhinoID	a		owl:DatatypeProperty ;
		rdfs:label	"reference to RhinoID"@en ,
				"refereert naar RhinoID"@nl ;
		
		rdfs:comment	"connects an instance with a Literal containing a RhinoID as a reference to the object representation in the stg:RhinoFile"@en ,
				"Verbindt een instantie met een Literal die de ruwe OBJ-serializatie ervan behelst"@nl ;

		rdfs:domain	geo:Geometry ;
		rdfs:range	stg:RhinoID .

stg:hasOrigin 	a 		owl:ObjectProperty ;
		rdfs:subClassOf geo:hasGeometry ;
		rdfs:label	"links to Project Origin"@en ;
		rdfs:domain	geo:Feature ;
		rdfs:range	stg:ProjectOrigin .

stg:hasModellingRemark a 	owl:ObjectProperty ;
		rdfs:label	"Modelling remark"@en ,
				"Modelleeropmerking"@nl ;

		rdfs:comment	"Statement about the geometry, such as metadata or an assumption that was made while modelling as-built geometry"@en ,
				"Opmerking over de geometrie, zoals metadata of een modelleerveronderstelling"@nl ;

		rdfs:domain	geo:Geometry ;
		rdfs:range 	stg:ModellingRemark .

stg:hasOcclusion a 	owl:ObjectProperty ;
		rdfs:label	"Occlusion"@en ,
				"Occlusion"@nl ;
		rdfs:subPropertyOf stg:hasModellingRemark ;
		rdfs:comment	"Defines a geometry as an occluded area"@en ,
				"Definieert een geometrie als een occluded area."@nl ;

		rdfs:domain	geo:Geometry ;
		rdfs:range 	stg:OccludedGeometry .

stg:hasLOA a 	owl:ObjectProperty ;
		rdfs:label	"Level of Accuracy"@en ,
				"Level of Accuracy"@nl ;
		rdfs:subPropertyOf stg:hasModellingRemark ;

		rdfs:comment	"States that a geometry has a certain (represented) LOA (USIBD definition)"@en ,
				"Linkt een geometrie aan een bepaalde (represented) LOA (zoals gedefinieerd door USIBD)."@nl ;

		rdfs:domain	geo:Geometry ;
		rdfs:range 	stg:LevelOfAccuracy .

stg:usedDeviationAnalysis a 	owl:DatatypeProperty ;
		rdfs:label	"Deviation Analysis"@en ;
		rdfs:comment	"States that a geometry has a certain (represented) LOA (USIBD definition)"@en ;

		rdfs:domain	stg:LevelOfAccuracy ;
		rdfs:range 	rdfs:Literal .

stg:usedEquipment a 	owl:DatatypeProperty ;
		rdfs:label	"Equipment"@en ;
		rdfs:comment	"Links a certain source to the equipment that was used for making this source. Currently this links to a Literal."@en ;

		rdfs:domain	stg:SourceFile ;
		rdfs:range 	rdfs:Literal .

stg:hasLOAvalue a 	owl:DatatypeProperty ;
		rdfs:label	"LOA value"@en ;
		rdfs:comment	"States the represented LOA value of a geometry after a geometric deviation analysis"@en ;

		rdfs:domain	stg:LevelOfAccuracy ;
		rdfs:range 	rdfs:Literal .

stg:denotesRemark	a	owl:DatatypeProperty ;
		rdfs:label	"reference to modelling remark"@en ,
				"refereert naar modelleeropmerking"@nl ;
		
		rdfs:comment	"connects a geometry with a Literal (string) that contains information about the modelling process"@en ,
				"Verbindt een geometrie met een Literal (string) die informatie over het modelleerprocess bevat"@nl ;

		rdfs:domain	geo:Geometry ;
		rdfs:range stg:Assumption .
